Code/HOL_Light/Lambda/dbmonad.ml
@@ -9,76 +9,76 @@
 (* ========================================================================= *)
 
 (* ------------------------------------------------------------------------- *)
-(* dB monads.                                                                *)
+(* Substoids (De Bruijn monads).                                             *)
 (* ------------------------------------------------------------------------- *)
 
-let DBMONAD_DEF = new_definition
+let SUBSTOID_DEF = new_definition
   `!op:(num->A)->A->A.
-     DBMONAD op <=>
+     SUBSTOID op <=>
      (!f g x. op g (op f x) = op (\n. op g (f n)) x) /\
      (?i. (!f n. op f (i n) = f n) /\ (!x. op i x = x))`;;
 
-let DBUNIT = new_definition
+let SBUNIT = new_definition
   `!op:(num->A)->A->A.
-     DBUNIT op = (@i. (!f n. op f (i n) = f n) /\ (!x. op i x = x))`;;
+     SBUNIT op = (@i. (!f n. op f (i n) = f n) /\ (!x. op i x = x))`;;
 
-let DBMONAD = prove
- (`!op. DBMONAD op <=>
+let SUBSTOID = prove
+ (`!op. SUBSTOID op <=>
         (!f g x:A. op g (op f x) = op (\n. op g (f n)) x) /\
-        (!f n. op f (DBUNIT op n) = f n) /\
-        (!x. op (DBUNIT op) x = x)`,
-  REWRITE_TAC[DBMONAD_DEF; DBUNIT] THEN MESON_TAC[]);;
+        (!f n. op f (SBUNIT op n) = f n) /\
+        (!x. op (SBUNIT op) x = x)`,
+  REWRITE_TAC[SUBSTOID_DEF; SBUNIT] THEN MESON_TAC[]);;
 
-let DBMONAD_ASSOC = prove
- (`!op. DBMONAD op ==> !f g x:A. op g (op f x) = op (op g o f) x`,
-  REWRITE_TAC[DBMONAD; o_DEF] THEN MESON_TAC[]);;
+let SUBSTOID_ASSOC = prove
+ (`!op. SUBSTOID op ==> !f g x:A. op g (op f x) = op (op g o f) x`,
+  REWRITE_TAC[SUBSTOID; o_DEF] THEN MESON_TAC[]);;
 
-let DBMONAD_RUNIT = prove
- (`!op. DBMONAD op ==> (!f n. op f (DBUNIT op n) = f n:A)`,
-  REWRITE_TAC[DBMONAD] THEN MESON_TAC[]);;
+let SUBSTOID_RUNIT = prove
+ (`!op. SUBSTOID op ==> (!f n. op f (SBUNIT op n) = f n:A)`,
+  REWRITE_TAC[SUBSTOID] THEN MESON_TAC[]);;
 
-let DBMONAD_LUNIT = prove
- (`!op. DBMONAD op ==> (!x:A. op (DBUNIT op) x = x)`,
-  REWRITE_TAC[DBMONAD] THEN MESON_TAC[]);;
+let SUBSTOID_LUNIT = prove
+ (`!op. SUBSTOID op ==> (!x:A. op (SBUNIT op) x = x)`,
+  REWRITE_TAC[SUBSTOID] THEN MESON_TAC[]);;
 
-let DBMONAD_LUNIT_IMP = prove
- (`!op f x:A. DBMONAD op /\ (!i. f i = DBUNIT op i) ==> op f x = x`,
+let SUBSTOID_LUNIT_IMP = prove
+ (`!op f x:A. SUBSTOID op /\ (!i. f i = SBUNIT op i) ==> op f x = x`,
   REPEAT GEN_TAC THEN REWRITE_TAC[GSYM FUN_EQ_THM; ETA_AX] THEN
-  SIMP_TAC[DBMONAD_LUNIT]);;
+  SIMP_TAC[SUBSTOID_LUNIT]);;
 
-let DBUNIT_UNIQUE = prove
- (`!op i. DBMONAD op /\ (!f n. op f (i n) = f n:A) /\ (!x. op i x = x)
-          ==> DBUNIT op = i`,
-  REWRITE_TAC[DBMONAD_DEF; DBUNIT; FUN_EQ_THM] THEN MESON_TAC[]);;
+let SBUNIT_UNIQUE = prove
+ (`!op i. SUBSTOID op /\ (!f n. op f (i n) = f n:A) /\ (!x. op i x = x)
+          ==> SBUNIT op = i`,
+  REWRITE_TAC[SUBSTOID_DEF; SBUNIT; FUN_EQ_THM] THEN MESON_TAC[]);;
 
 (* ------------------------------------------------------------------------- *)
 (* Free variables.                                                           *)
 (* ------------------------------------------------------------------------- *)
 
 (*
-let DBFREES = new_definition
-  `DBFREES (op:(num->A)->A->A) x =
-   INTERS {s | !f. (!i. i IN s ==> f i = DBUNIT op i) ==> op f x = x}`;;
+let SBFREE = new_definition
+  `SBFREE (op:(num->A)->A->A) x =
+   INTERS {s | !f. (!i. i IN s ==> f i = SBUNIT op i) ==> op f x = x}`;;
 
-let DBFREES' = new_definition
-  `DBFREES' (op:(num->A)->A->A) x =
-   {i | !f. (!j. ~(j = i) ==> f j = DBUNIT op j) ==> op f x = x}`;;
+let SBFREE' = new_definition
+  `SBFREE' (op:(num->A)->A->A) x =
+   {i | !f. (!j. ~(j = i) ==> f j = SBUNIT op j) ==> op f x = x}`;;
 
-let DBMONAD_LUNIT_FUN = prove
- (`!f x:A. (!i. i IN DBFREES' op x ==> f i = DBUNIT op i) ==> op f x = x`,
+let SUBSTOID_LUNIT_FUN = prove
+ (`!f x:A. (!i. i IN SBFREE' op x ==> f i = SBUNIT op i) ==> op f x = x`,
   REPEAT GEN_TAC THEN
-  REWRITE_TAC[DBFREES'] THEN
+  REWRITE_TAC[SBFREE'] THEN
   REWRITE_TAC[FORALL_IN_GSPEC] THEN
   DISCH_TAC THEN
 
-let DBMONAD_EXTENS = prove
- (`!op f g x:A. DBMONAD op /\ (!i. i IN DBFREES' op x ==> f i = g i)
+let SUBSTOID_EXTENS = prove
+ (`!op f g x:A. SUBSTOID op /\ (!i. i IN SBFREE' op x ==> f i = g i)
                 ==> op f x = op g x`,
 
   REPEAT STRIP_TAC THEN
   ABBREV_TAC `s = {i:num | f i:A = g i}`
-  CLAIM_TAC "rmk" `s SUBSET DBFREES' op (x:A)`
-  REWRITE_TAC[DBFREES'; SUBSET] THEN
+  CLAIM_TAC "rmk" `s SUBSET SBFREE' op (x:A)`
+  REWRITE_TAC[SBFREE'; SUBSET] THEN
   POP_ASSUM SUBST_VAR_TAC THEN
   REWRITE_TAC[FORALL_IN_GSPEC] THEN
   INTRO_TAC "!i; eq" THEN
@@ -88,199 +88,199 @@ let DBMONAD_EXTENS = prove
 *)
 
 (* ------------------------------------------------------------------------- *)
-(* DBREINDEX                                                                 *)
+(* SBREINDEX                                                                 *)
 (* ------------------------------------------------------------------------- *)
 
-let DBREINDEX = new_definition
-  `DBREINDEX op f x:A = op (DBUNIT op o f) x`;;
+let SBREINDEX = new_definition
+  `SBREINDEX op f x:A = op (SBUNIT op o f) x`;;
 
-let DBREINDEX_DBREINDEX = prove
+let SBREINDEX_SBREINDEX = prove
  (`!op f g x:A.
-     DBMONAD op
-     ==> DBREINDEX op g (DBREINDEX op f x) = DBREINDEX op (g o f) x`,
-  REPEAT GEN_TAC THEN DISCH_TAC THEN REWRITE_TAC[DBREINDEX] THEN
-  ASM_SIMP_TAC[DBMONAD_ASSOC] THEN AP_THM_TAC THEN AP_TERM_TAC THEN
-  ASM_SIMP_TAC[DBMONAD_RUNIT; FUN_EQ_THM; o_THM]);;
+     SUBSTOID op
+     ==> SBREINDEX op g (SBREINDEX op f x) = SBREINDEX op (g o f) x`,
+  REPEAT GEN_TAC THEN DISCH_TAC THEN REWRITE_TAC[SBREINDEX] THEN
+  ASM_SIMP_TAC[SUBSTOID_ASSOC] THEN AP_THM_TAC THEN AP_TERM_TAC THEN
+  ASM_SIMP_TAC[SUBSTOID_RUNIT; FUN_EQ_THM; o_THM]);;
 
-let DBREINDEX_DBUNIT = prove
- (`!op f i. DBMONAD op ==> DBREINDEX op f (DBUNIT op i) = DBUNIT op (f i):A`,
-  REPEAT GEN_TAC THEN DISCH_TAC THEN REWRITE_TAC[DBREINDEX] THEN
-  ASM_SIMP_TAC[DBMONAD_RUNIT] THEN REWRITE_TAC[o_THM]);;
+let SBREINDEX_SBUNIT = prove
+ (`!op f i. SUBSTOID op ==> SBREINDEX op f (SBUNIT op i) = SBUNIT op (f i):A`,
+  REPEAT GEN_TAC THEN DISCH_TAC THEN REWRITE_TAC[SBREINDEX] THEN
+  ASM_SIMP_TAC[SUBSTOID_RUNIT] THEN REWRITE_TAC[o_THM]);;
 
-let DBREINDEX_DBSUBST = prove
- (`!op f g x:A. DBMONAD op
-                ==> DBREINDEX op f (op g x) = op (DBREINDEX op f o g) x`,
+let SBREINDEX_DBSUBST = prove
+ (`!op f g x:A. SUBSTOID op
+                ==> SBREINDEX op f (op g x) = op (SBREINDEX op f o g) x`,
   REPEAT GEN_TAC THEN DISCH_TAC THEN
-  ASM_SIMP_TAC[DBREINDEX; DBMONAD_ASSOC; o_THM] THEN
-  AP_THM_TAC THEN AP_TERM_TAC THEN REWRITE_TAC[FUN_EQ_THM; o_THM; DBREINDEX]);;
+  ASM_SIMP_TAC[SBREINDEX; SUBSTOID_ASSOC; o_THM] THEN
+  AP_THM_TAC THEN AP_TERM_TAC THEN REWRITE_TAC[FUN_EQ_THM; o_THM; SBREINDEX]);;
 
-let DBSUBST_DBREINDEX = prove
- (`!op f g x:A. DBMONAD op ==> op f (DBREINDEX op g x) = op (f o g) x`,
-  REPEAT GEN_TAC THEN DISCH_TAC THEN REWRITE_TAC[DBREINDEX] THEN
-  ASM_SIMP_TAC[DBMONAD_ASSOC] THEN AP_THM_TAC THEN AP_TERM_TAC THEN
+let DBSUBST_SBREINDEX = prove
+ (`!op f g x:A. SUBSTOID op ==> op f (SBREINDEX op g x) = op (f o g) x`,
+  REPEAT GEN_TAC THEN DISCH_TAC THEN REWRITE_TAC[SBREINDEX] THEN
+  ASM_SIMP_TAC[SUBSTOID_ASSOC] THEN AP_THM_TAC THEN AP_TERM_TAC THEN
   REWRITE_TAC[FUN_EQ_THM; o_THM] THEN GEN_TAC THEN
-  ASM_SIMP_TAC[DBMONAD_RUNIT]);;
+  ASM_SIMP_TAC[SUBSTOID_RUNIT]);;
 
 (* ------------------------------------------------------------------------- *)
 (* Morphisms of dB-monads.                                                   *)
 (* ------------------------------------------------------------------------- *)
 
-let DBMONAD_MOR = new_definition
+let SUBSTOID_MOR = new_definition
   `!op1 op2 h:A->B.
-     DBMONAD_MOR op1 op2 h <=>
-     DBMONAD op1 /\ DBMONAD op2 /\
-     (!n. h (DBUNIT op1 n) = DBUNIT op2 n) /\
+     SUBSTOID_MOR op1 op2 h <=>
+     SUBSTOID op1 /\ SUBSTOID op2 /\
+     (!n. h (SBUNIT op1 n) = SBUNIT op2 n) /\
      (!f x. h (op1 f x) = op2 (h o f) (h x))`;;
 
-let DBMONAD_MOR_THM = prove
- (`(!op1 op2 h:A->B. DBMONAD_MOR op1 op2 h ==> DBMONAD op1) /\
-   (!op1 op2 h:A->B. DBMONAD_MOR op1 op2 h ==> DBMONAD op2) /\
-   (!op1 op2 h:A->B. DBMONAD_MOR op1 op2 h
-                     ==> (!n. h (DBUNIT op1 n) = DBUNIT op2 n)) /\
-   (!op1 op2 h:A->B. DBMONAD_MOR op1 op2 h
+let SUBSTOID_MOR_THM = prove
+ (`(!op1 op2 h:A->B. SUBSTOID_MOR op1 op2 h ==> SUBSTOID op1) /\
+   (!op1 op2 h:A->B. SUBSTOID_MOR op1 op2 h ==> SUBSTOID op2) /\
+   (!op1 op2 h:A->B. SUBSTOID_MOR op1 op2 h
+                     ==> (!n. h (SBUNIT op1 n) = SBUNIT op2 n)) /\
+   (!op1 op2 h:A->B. SUBSTOID_MOR op1 op2 h
                      ==> (!f x. h (op1 f x) = op2 (h o f) (h x)))`,
-  REWRITE_TAC[DBMONAD_MOR] THEN MESON_TAC[]);;
+  REWRITE_TAC[SUBSTOID_MOR] THEN MESON_TAC[]);;
 
-let DBMONAD_MOR_ID = prove
- (`!op:(num->A)->A->A. DBMONAD op ==> DBMONAD_MOR op op I`,
-  REWRITE_TAC[DBMONAD_MOR; I_THM; I_O_ID]);;
+let SUBSTOID_MOR_ID = prove
+ (`!op:(num->A)->A->A. SUBSTOID op ==> SUBSTOID_MOR op op I`,
+  REWRITE_TAC[SUBSTOID_MOR; I_THM; I_O_ID]);;
 
-let DBMONAD_MOR_o = prove
+let SUBSTOID_MOR_o = prove
  (`!op1 op2 op3 h:A->B g:B->C.
-     DBMONAD_MOR op1 op2 h /\ DBMONAD_MOR op2 op3 g
-     ==> DBMONAD_MOR op1 op3 (g o h)`,
-  REPEAT GEN_TAC THEN REWRITE_TAC[DBMONAD_MOR] THEN STRIP_TAC THEN
+     SUBSTOID_MOR op1 op2 h /\ SUBSTOID_MOR op2 op3 g
+     ==> SUBSTOID_MOR op1 op3 (g o h)`,
+  REPEAT GEN_TAC THEN REWRITE_TAC[SUBSTOID_MOR] THEN STRIP_TAC THEN
   ASM_REWRITE_TAC[o_THM; o_ASSOC]);;
 
-let DBMONAD_MOR_IMP = MATCH_MP EQ_IMP (SPEC_ALL DBMONAD_MOR);;
+let SUBSTOID_MOR_IMP = MATCH_MP EQ_IMP (SPEC_ALL SUBSTOID_MOR);;
 
 (* ------------------------------------------------------------------------- *)
-(*  Modules.                                                                 *)
+(*  Substoid modules.                                                        *)
 (* ------------------------------------------------------------------------- *)
 
-let MODULE_DEF = new_definition
+let SBMODULE_DEF = new_definition
   `!op mop:(num->A)->B->B.
-     MODULE op mop <=> DBMONAD op /\
-                       (!x. mop (DBUNIT op) x = x) /\
+     SBMODULE op mop <=> SUBSTOID op /\
+                       (!x. mop (SBUNIT op) x = x) /\
                        (!f g x. mop g (mop f x) = mop (op g o f) x)`;;
 
-let SELF_DBMODULE = prove
- (`!op:(num->A)->A->A. MODULE op op <=> DBMONAD op`,
-  REWRITE_TAC[DBMONAD; MODULE_DEF; o_DEF] THEN MESON_TAC[]);;
+let SELF_SBMODULE = prove
+ (`!op:(num->A)->A->A. SBMODULE op op <=> SUBSTOID op`,
+  REWRITE_TAC[SUBSTOID; SBMODULE_DEF; o_DEF] THEN MESON_TAC[]);;
 
-let MODULE_MOR = new_definition
+let SBMODULE_MOR = new_definition
   `!op mop1 mop2 h.
-     MODULE_MOR op mop1 mop2 h <=>
-     MODULE op mop1 /\
-     MODULE op mop2 /\
+     SBMODULE_MOR op mop1 mop2 h <=>
+     SBMODULE op mop1 /\
+     SBMODULE op mop2 /\
      (!f:num->A x:M. h (mop1 f x) = mop2 f (h x):N)`;;
 
-let MODULE_MOR_ID = prove
- (`!op mop:(num->A)->B->B. MODULE op mop <=> MODULE_MOR op mop mop I`,
-  REWRITE_TAC[MODULE_MOR; I_THM]);;
+let SBMODULE_MOR_ID = prove
+ (`!op mop:(num->A)->B->B. SBMODULE op mop <=> SBMODULE_MOR op mop mop I`,
+  REWRITE_TAC[SBMODULE_MOR; I_THM]);;
 
-let MODULE_MOR_o = prove
+let SBMODULE_MOR_o = prove
  (`!op:(num->A)->A->A mop1 mop2 g:N->L h:M->N.
-     MODULE_MOR op mop1 mop2 h /\ MODULE_MOR op mop2 mop3 g
-     ==> MODULE_MOR op mop1 mop3 (g o h)`,
-  REWRITE_TAC[MODULE_MOR] THEN REPEAT STRIP_TAC THEN
+     SBMODULE_MOR op mop1 mop2 h /\ SBMODULE_MOR op mop2 mop3 g
+     ==> SBMODULE_MOR op mop1 mop3 (g o h)`,
+  REWRITE_TAC[SBMODULE_MOR] THEN REPEAT STRIP_TAC THEN
   ASM_REWRITE_TAC[o_DEF]);;
 
 (* ------------------------------------------------------------------------- *)
-(*  Pull-back modules.                                                       *)
+(*  Pull-back SBMODULEs.                                                       *)
 (* ------------------------------------------------------------------------- *)
 
 let PBMOP = new_definition
   `!op':(num->A')->A'->A' op:(num->A)->A->A h:A'->A mop:(num->A)->M->M f.
      PBMOP op' op h mop f = mop (h o f)`;;
 
-let PB_DBMODULE = prove
+let PB_SBMODULE = prove
  (`!op' op h:A'->A mop:(num->A)->M->M.
-      DBMONAD_MOR op' op h /\ MODULE op mop
-      ==> MODULE op' (PBMOP op' op h mop)`,
-  REWRITE_TAC[DBMONAD_MOR; MODULE_DEF; PBMOP] THEN REPEAT STRIP_TAC THEN
+      SUBSTOID_MOR op' op h /\ SBMODULE op mop
+      ==> SBMODULE op' (PBMOP op' op h mop)`,
+  REWRITE_TAC[SUBSTOID_MOR; SBMODULE_DEF; PBMOP] THEN REPEAT STRIP_TAC THEN
   ASM_REWRITE_TAC[o_DEF; ETA_AX]);;
 
 (* ------------------------------------------------------------------------- *)
-(*  Derived Modules.                                                         *)
+(*  Derived SBMODULEs.                                                         *)
 (* ------------------------------------------------------------------------- *)
 
-let DBDERIV = new_recursive_definition num_RECURSION
-  `(!op f. DBDERIV op f 0 = DBUNIT op 0:A) /\
-   (!op f i. DBDERIV op f (SUC i) = DBREINDEX op SUC (f i))`;;
+let SBDERIV = new_recursive_definition num_RECURSION
+  `(!op f. SBDERIV op f 0 = SBUNIT op 0:A) /\
+   (!op f i. SBDERIV op f (SUC i) = SBREINDEX op SUC (f i))`;;
 
-let DBDERIV_DBUNIT = prove
- (`!op. DBMONAD op ==> DBDERIV op (DBUNIT op) = DBUNIT op:num->A`,
+let SBDERIV_SBUNIT = prove
+ (`!op. SUBSTOID op ==> SBDERIV op (SBUNIT op) = SBUNIT op:num->A`,
   GEN_TAC THEN DISCH_TAC THEN REWRITE_TAC[FUN_EQ_THM] THEN NUM_CASES_TAC THEN
-  REWRITE_TAC[DBDERIV] THEN ASM_SIMP_TAC[DBREINDEX_DBUNIT]);;
+  REWRITE_TAC[SBDERIV] THEN ASM_SIMP_TAC[SBREINDEX_SBUNIT]);;
 
 let DMOP = new_definition
   `!op:(num->A)->A->A mop:(num->A)->M->M f:num->A x:M.
-     DMOP op mop f x = mop (DBDERIV op f) x:M`;;
+     DMOP op mop f x = mop (SBDERIV op f) x:M`;;
 
-let MODULE_DMOP = prove
- (`!op mop:(num->A)->M->M. MODULE op mop ==> MODULE op (DMOP op mop)`,
+let SBMODULE_DMOP = prove
+ (`!op mop:(num->A)->M->M. SBMODULE op mop ==> SBMODULE op (DMOP op mop)`,
   REPEAT GEN_TAC THEN INTRO_TAC "mod" THEN
-  HYP_TAC "mod -> mnd munit massoc" (REWRITE_RULE[MODULE_DEF]) THEN
-  ASM_REWRITE_TAC[MODULE_DEF] THEN REPEAT STRIP_TAC THEN
-  REWRITE_TAC[DMOP] THEN ASM_SIMP_TAC[DBDERIV_DBUNIT] THEN
+  HYP_TAC "mod -> mnd munit massoc" (REWRITE_RULE[SBMODULE_DEF]) THEN
+  ASM_REWRITE_TAC[SBMODULE_DEF] THEN REPEAT STRIP_TAC THEN
+  REWRITE_TAC[DMOP] THEN ASM_SIMP_TAC[SBDERIV_SBUNIT] THEN
   REWRITE_TAC[o_THM] THEN AP_THM_TAC THEN AP_TERM_TAC THEN
   REWRITE_TAC[FUN_EQ_THM] THEN NUM_CASES_TAC THEN
-  ASM_SIMP_TAC[DBDERIV; DBMONAD_RUNIT; o_THM] THEN
-  ASM_SIMP_TAC[DBSUBST_DBREINDEX; DBREINDEX_DBSUBST] THEN
-  AP_THM_TAC THEN AP_TERM_TAC THEN REWRITE_TAC[FUN_EQ_THM; o_THM; DBDERIV]);;
+  ASM_SIMP_TAC[SBDERIV; SUBSTOID_RUNIT; o_THM] THEN
+  ASM_SIMP_TAC[DBSUBST_SBREINDEX; SBREINDEX_DBSUBST] THEN
+  AP_THM_TAC THEN AP_TERM_TAC THEN REWRITE_TAC[FUN_EQ_THM; o_THM; SBDERIV]);;
 
-let MODULE_DMOP_MOR = prove
+let SBMODULE_DMOP_MOR = prove
  (`!op:(num->A)->A->A mop1 mop2 h:M->N.
-     MODULE_MOR op mop1 mop2 h
-     ==> MODULE_MOR op (DMOP op mop1) (DMOP op mop2) h`,
-  SIMP_TAC[MODULE_MOR; MODULE_DMOP; DMOP]);;
+     SBMODULE_MOR op mop1 mop2 h
+     ==> SBMODULE_MOR op (DMOP op mop1) (DMOP op mop2) h`,
+  SIMP_TAC[SBMODULE_MOR; SBMODULE_DMOP; DMOP]);;
 
-let MODULE_MOR_INV = prove
+let SBMODULE_MOR_INV = prove
  (`!op:(num->A)->A->A mop1 mop2 g:M->N h:N->M.
-     MODULE_MOR op mop1 mop2 h /\
+     SBMODULE_MOR op mop1 mop2 h /\
      (!x. g (h x) = x) /\ (!y. h (g y) = y)
-     ==> MODULE_MOR op mop2 mop1 g`,
-  REWRITE_TAC[MODULE_MOR] THEN MESON_TAC[]);;
+     ==> SBMODULE_MOR op mop2 mop1 g`,
+  REWRITE_TAC[SBMODULE_MOR] THEN MESON_TAC[]);;
 
-let MODULE_ISOM = new_definition
+let SBMODULE_ISOM = new_definition
   `!op:(num->A)->A->A mop1 mop2 h:M->N g:N->M.
-     MODULE_ISOM op mop1 mop2 h g <=>
-       MODULE_MOR op mop1 mop2 h /\
+     SBMODULE_ISOM op mop1 mop2 h g <=>
+       SBMODULE_MOR op mop1 mop2 h /\
        (!x. g (h x) = x) /\ (!y. h (g y) = y)`;;
 
-let MODULE_ISOM_SYM = prove
+let SBMODULE_ISOM_SYM = prove
  (`!op:(num->A)->A->A mop1 mop2 h:M->N g:N->M.
-     MODULE_ISOM op mop1 mop2 h g
-     ==> MODULE_ISOM op mop2 mop1 g h`,
-  REWRITE_TAC[MODULE_ISOM] THEN REPEAT STRIP_TAC THEN
-  ASM_REWRITE_TAC[] THEN MATCH_MP_TAC MODULE_MOR_INV THEN
+     SBMODULE_ISOM op mop1 mop2 h g
+     ==> SBMODULE_ISOM op mop2 mop1 g h`,
+  REWRITE_TAC[SBMODULE_ISOM] THEN REPEAT STRIP_TAC THEN
+  ASM_REWRITE_TAC[] THEN MATCH_MP_TAC SBMODULE_MOR_INV THEN
   ASM_MESON_TAC[]);;
 
-let MODULE_ISOM_UNFOLD = prove
+let SBMODULE_ISOM_UNFOLD = prove
  (`!op:(num->A)->A->A mop1 mop2 h:M->N g.
-     MODULE_ISOM op mop1 mop2 h g <=>
-     MODULE op mop1 /\
-     MODULE op mop2 /\
-     MODULE_MOR op mop1 mop2 h /\
-     MODULE_MOR op mop2 mop1 g /\
+     SBMODULE_ISOM op mop1 mop2 h g <=>
+     SBMODULE op mop1 /\
+     SBMODULE op mop2 /\
+     SBMODULE_MOR op mop1 mop2 h /\
+     SBMODULE_MOR op mop2 mop1 g /\
      (!x. g (h x) = x) /\ (!y. h (g y) = y)`,
   REPEAT GEN_TAC THEN EQ_TAC THEN STRIP_TAC THENL
-  [ALL_TAC; ASM_REWRITE_TAC[MODULE_ISOM]] THEN
-  FIRST_ASSUM (ASSUME_TAC o MATCH_MP MODULE_ISOM_SYM) THEN
-  RULE_ASSUM_TAC (REWRITE_RULE [MODULE_ISOM]) THEN
+  [ALL_TAC; ASM_REWRITE_TAC[SBMODULE_ISOM]] THEN
+  FIRST_ASSUM (ASSUME_TAC o MATCH_MP SBMODULE_ISOM_SYM) THEN
+  RULE_ASSUM_TAC (REWRITE_RULE [SBMODULE_ISOM]) THEN
   ASM_REWRITE_TAC[] THEN
-  RULE_ASSUM_TAC (REWRITE_RULE [MODULE_MOR]) THEN
+  RULE_ASSUM_TAC (REWRITE_RULE [SBMODULE_MOR]) THEN
   ASM_REWRITE_TAC[]);;
 
-let EXP_DBMONAD = new_definition
+let EXP_SUBSTOID = new_definition
   `!op:(num->A)->A->A h g.
-     EXP_DBMONAD op h g <=> MODULE_ISOM op op (DMOP op op) h g`;;
+     EXP_SUBSTOID op h g <=> SBMODULE_ISOM op op (DMOP op op) h g`;;
 
-let EXP_DBMONAD_MOR = new_definition
+let EXP_SUBSTOID_MOR = new_definition
   `!op1 h1 g1 op2 h2 g2 f:A->B.
-     EXP_DBMONAD_MOR op1 h1 g1 op2 h2 g2 f <=>
-     EXP_DBMONAD op1 h1 g1 /\
-     EXP_DBMONAD op2 h2 g2 /\
-     DBMONAD_MOR op1 op2 f /\
+     EXP_SUBSTOID_MOR op1 h1 g1 op2 h2 g2 f <=>
+     EXP_SUBSTOID op1 h1 g1 /\
+     EXP_SUBSTOID op2 h2 g2 /\
+     SUBSTOID_MOR op1 op2 f /\
       (!x. h2 (f x) = f (h1 x))`;;
